renamed sum to sum_of_nats

acl2/books/erl-arithmetic/sum_of_nats.lisp
@@ -3,11 +3,11 @@
 
 (set-induction-depth-limit 1)
 
-; ACL2 sum
-(define sum ((n natp))
+; ACL2 sum_of_nats
+(define sum-of-nats ((n natp))
   (b* ((n (nfix n))
        ((if (= n 0)) 0))
-      (+ n (sum (1- n)))))
+      (+ n (sum-of-nats (1- n)))))
 
 ;; An Erlang World with the following functions defined locally:
 ;; - Remark: When Erlang is run on the command line, the module is set to 'local.
@@ -15,8 +15,8 @@
 ;;   which we would then have to import (or do a remote call [m:f()]) but I will
 ;;   ignore that here for simplicity by defining [add] in the local module.
 ;;
-;; sum(0) -> 0;
-;; sum(X) when is_integer(X), X > 0 -> X + sum(X - 1).
+;; sum_of_nats(0) -> 0;
+;; sum_of_nats(X) when is_integer(X), X > 0 -> X + sum_of_nats(X - 1).
 ;;
 (define sum-test-w ()
   :returns (w world-p)
@@ -26,25 +26,25 @@
              (export)
              (import))
       (fn-defns
-        (((name . sum) (arity . 1)) ;; sum(0) -> 0;
+        (((name . sum_of_nats) (arity . 1)) ;; sum_of_nats(0) -> 0;
          ((cases (:integer 0))
           (guards)
           (body (:integer 0)))
-         ((cases (:var X)) ;; sum(X) when is_integer(X), X > 0 -> X + sum(X - 1).
+         ((cases (:var X)) ;; sum_of_nats(X) when is_integer(X), X > 0 -> X + sum_of_nats(X - 1).
           (guards ((:call is_integer (:cons (:var X) (:nil))) 
                    (:binop > (:var X) (:integer 0))))
           (body (:binop
                   +
                   (:var X) 
                   (:call 
-                    sum
+                    sum_of_nats
                     (:cons (:binop - (:var X) (:integer 1)) 
                            (:nil)))))))))))
 
 ; While it is not necessary to admit the theorem below, this lemma speeds up 
 ; the proof quite a bit. ACL2 has an easier time dealing with the cases of 
 ; eval-local-call and apply-k separately.
-(defrule local-call-of-sum
+(defrule local-call-of-sum-of-nats
   (implies
     (and 
       (wf-state-p s)
@@ -55,7 +55,7 @@
       (not (cdr args))
       (equal (erl-val-kind (car args)) :integer))
     (equal 
-      (eval-local-call s 'sum args)
+      (eval-local-call s 'sum_of_nats args)
       (if (> (erl-val-integer->val (car args)) 0)
           (mv (update-erl-state->bind
                 (update-erl-state->in s (car args))
@@ -64,7 +64,7 @@
                   + 
                   (:var X) 
                   (:call 
-                    sum 
+                    sum_of_nats 
                     (:cons (:binop - (:var X) (:integer 1)) 
                             (:nil))))))
           (if (equal (erl-val-integer->val (car args)) 0)
@@ -86,7 +86,7 @@
      eval-guard eval-guard-expr eval-bif apply-erl-binop
      apply-erl-comp-binop erl-compare))
 
-; Induction schema for apply-k-of-sum
+; Induction schema for apply-k-of-sum-of-nats
 (local (define apply-k-of-sum-induct (args k)
   (declare (irrelevant k))
   :measure 
@@ -114,10 +114,10 @@
                             (car (erl-val-cons->lst (erl-state->in args)))
                             nil))
             (erl-k (+ -5 (erl-k->fuel k))
-                        '(:local-call sum)))))))
+                        '(:local-call sum_of_nats)))))))
 
-; Base case of calling apply-k with sum
-(defrule apply-k-of-sum-base-case
+; Base case of calling apply-k with sum_of_nats
+(defrule apply-k-of-sum-of-nats-base-case
   (implies 
     (and
       (wf-state-p s)
@@ -127,9 +127,9 @@
       (equal (erl-state->world s) (sum-test-w))
       (equal (erl-state->module s) 'local)
       
-      ; the next continuation is a call to [sum]
+      ; the next continuation is a call to [sum_of_nats]
       (equal (kont-kind (erl-k->kont k)) :local-call)
-      (equal (kont-local-call->call (erl-k->kont k)) 'sum)
+      (equal (kont-local-call->call (erl-k->kont k)) 'sum_of_nats)
       
       ; the arguments are well-formed
       (equal (erl-val-kind (erl-state->in s)) :cons)
@@ -157,9 +157,9 @@
       (equal (erl-state->world s) (sum-test-w))
       (equal (erl-state->module s) 'local)
       
-      ; the next continuation is a call to [sum]
+      ; the next continuation is a call to [sum_of_nats]
       (equal (kont-kind (erl-k->kont k)) :local-call)
-      (equal (kont-local-call->call (erl-k->kont k)) 'sum)
+      (equal (kont-local-call->call (erl-k->kont k)) 'sum_of_nats)
       
       ; the arguments are well-formed
       (equal (erl-val-kind (erl-state->in s)) :cons)
@@ -186,7 +186,7 @@
                          (car (erl-val-cons->lst (erl-state->in s)))
                          nil))
          (list (erl-k (+ -5 (erl-k->fuel k))
-                     '(:local-call sum))))))
+                     '(:local-call sum_of_nats))))))
   :use ((:instance apply-k-of-local-call-when-match))
   :enable (apply-k-of-binop-expr1 apply-k-of-cons))
 
@@ -203,9 +203,9 @@
       (equal (erl-state->world s) (sum-test-w))
       (equal (erl-state->module s) 'local)
       
-      ; the next continuation is a call to [sum]
+      ; the next continuation is a call to [sum_of_nats]
       (equal (kont-kind (erl-k->kont k)) :local-call)
-      (equal (kont-local-call->call (erl-k->kont k)) 'sum)
+      (equal (kont-local-call->call (erl-k->kont k)) 'sum_of_nats)
       
       ; the arguments are well-formed
       (wf-state-p s)
@@ -217,7 +217,7 @@
       ; the first (and only) argument is greater than or equal to 0.
       (> (erl-val-integer->val (car (erl-val-cons->lst (erl-state->in s)))) 0)
     
-      ; Let's assume the result is well-formed
+      ; Let's assumse the result is well-formed
       (wf-state-p (apply-k s (cons k nil))))
     (equal (erl-state->in (apply-k s (cons k nil)))
            (apply-erl-binop
@@ -237,9 +237,9 @@
                                   (car (erl-val-cons->lst (erl-state->in s)))
                                   nil))
                   (list (erl-k (+ -5 (erl-k->fuel k))
-                               '(:local-call sum))))))))
+                               '(:local-call sum_of_nats))))))))
   
-  :disable (inductive-step-is-wf apply-k-of-sum-base-case)
+  :disable (inductive-step-is-wf apply-k-of-sum-of-nats-base-case)
   :enable (apply-k-of-binop-expr1 apply-k-of-cons)
 
   ; this case split can be removed by proving a lemma regarding
@@ -260,7 +260,7 @@
                                 (car (erl-val-cons->lst (erl-state->in s)))
                                 nil))
                 (list (erl-k (+ -5 (erl-k->fuel k))
-                            '(:local-call sum)))))
+                            '(:local-call sum_of_nats)))))
             (omap::update 'x
                 (car (erl-val-cons->lst (erl-state->in s)))
                 nil)))
@@ -270,26 +270,26 @@
           ("Subgoal 1.1.1.1.1.1'"
             :cases ((equal
                       (erl-val-kind
-                        (ERL-STATE->IN
-                          (APPLY-K
-                            (UPDATE-ERL-STATE->BIND
-                            (UPDATE-ERL-STATE->IN
-                              S
-                              (ERL-VAL-CONS
-                              (LIST
-                                (ERL-VAL-INTEGER
+                        (erl-state->in
+                          (apply-k
+                            (update-erl-state->bind
+                            (update-erl-state->in
+                              s
+                              (erl-val-cons
+                              (list
+                                (erl-val-integer
                                       (+ -1
-                                        (ERL-VAL-INTEGER->VAL
-                                              (CAR (ERL-VAL-CONS->LST (ERL-STATE->IN S)))))))))
-                            (OMAP::UPDATE 'X
-                                          (CAR (ERL-VAL-CONS->LST (ERL-STATE->IN S)))
-                                          NIL))
-                            (LIST (ERL-K (+ -5 (ERL-K->FUEL K))
-                                        '(:LOCAL-CALL SUM))))))
+                                        (erl-val-integer->val
+                                              (car (erl-val-cons->lst (erl-state->in s)))))))))
+                            (omap::update 'X
+                                          (car (erl-val-cons->lst (erl-state->in s)))
+                                          nil))
+                            (list (erl-k (+ -5 (erl-k->fuel k))
+                                        '(:local-call sum_of_nats))))))
                       :integer)))))
 
-; Erlang sum is equivalent to the ACL2 sum, if evaluation succeeds.
-(defrule apply-k-of-sum
+; Erlang sum_of_nats is equivalent to the ACL2 sum-of-nats, if evaluation succeeds.
+(defrule apply-k-of-sum-of-nats
   (implies 
     (and
       ; there is enough fuel for each recursive call
@@ -299,9 +299,9 @@
       (equal (erl-state->world s) (sum-test-w))
       (equal (erl-state->module s) 'local)
       
-      ; the next continuation is a call to [sum]
+      ; the next continuation is a call to [sum_of_nats]
       (equal (kont-kind (erl-k->kont k)) :local-call)
-      (equal (kont-local-call->call (erl-k->kont k)) 'sum)
+      (equal (kont-local-call->call (erl-k->kont k)) 'sum_of_nats)
       
       ; the arguments are well-formed
       (wf-state-p s)
@@ -313,19 +313,20 @@
       ; the first (and only) argument is greater than or equal to 0.
       (>= (erl-val-integer->val (car (erl-val-cons->lst (erl-state->in s)))) 0)
       
-      ; Let's assume the result is well-formed
+      ; Let's assum_of_natse the result is well-formed
       (wf-state-p (apply-k s (cons k nil))))
     (equal
       (erl-state->in (apply-k s (cons k nil)))
       (make-erl-val-integer 
         :val
-          (sum (erl-val-integer->val 
-                 (car (erl-val-cons->lst (erl-state->in s))))))))
+          (sum-of-nats
+            (erl-val-integer->val 
+              (car (erl-val-cons->lst (erl-state->in s))))))))
   :induct (apply-k-of-sum-induct s k)
-  :in-theory (enable sum))
+  :in-theory (enable sum-of-nats))
 
 ; helper to simplify the above theorem (just replaces the argument with x).
-(defrule apply-k-of-sum-of-x
+(defrule apply-k-of-sum-of-nats-of-x
   (implies 
     (and
       (equal (* 8 (+ x 2)) (erl-k->fuel k))
@@ -333,9 +334,9 @@
       (equal (erl-state->world s) (sum-test-w))
       (equal (erl-state->module s) 'local)
       
-      ; the next continuation is a call to [sum]
+      ; the next continuation is a call to [sum_of_nats]
       (equal (kont-kind (erl-k->kont k)) :local-call)
-      (equal (kont-local-call->call (erl-k->kont k)) 'sum)
+      (equal (kont-local-call->call (erl-k->kont k)) 'sum_of_nats)
       
       ; the arguments are well-formed
       (equal (erl-val-kind (erl-state->in s)) :cons)
@@ -352,20 +353,21 @@
     (equal
       (erl-state->in (apply-k s (cons k nil)))
       (make-erl-val-integer 
-        :val (sum x))))
+        :val (sum-of-nats x))))
   :do-not-induct t
-  :disable apply-k-of-sum
-  :use (:instance apply-k-of-sum (s s) (k k)))
+  :disable apply-k-of-sum-of-nats
+  :use (:instance apply-k-of-sum-of-nats (s s) (k k)))
 
 
-; We can now use the existing ACL2 arithemtic books to reason about the sum function!
+; We can now use the existing ACL2 arithemtic books to reason about the sum_of_nats function!
 (include-book "arithmetic/top" :dir :system)
 
+; closed form of sum of nats
 (defrule cfs 
-    (implies (natp n) (equal (sum n) (/ (* n (+ n 1)) 2)))
-    :enable sum)
+    (implies (natp n) (equal (sum-of-nats n) (/ (* n (+ n 1)) 2)))
+    :enable sum-of-nats)
 
-(defrule apply-k-of-sum-closed-form
+(defrule apply-k-of-sum-of-nats-closed-form
   (implies 
     (and
       (equal (* 8 (+ x 2)) (erl-k->fuel k))
@@ -373,9 +375,9 @@
       (equal (erl-state->world s) (sum-test-w))
       (equal (erl-state->module s) 'local)
       
-      ; the next continuation is a call to [sum]
+      ; the next continuation is a call to [sum_of_nats]
       (equal (kont-kind (erl-k->kont k)) :local-call)
-      (equal (kont-local-call->call (erl-k->kont k)) 'sum)
+      (equal (kont-local-call->call (erl-k->kont k)) 'sum_of_nats)
       
       ; the arguments are well-formed
       (equal (erl-val-kind (erl-state->in s)) :cons)
@@ -385,7 +387,8 @@
 
       ; the first (and only) argument is a natp
       (natp x)
-      (equal (erl-val-integer->val (car (erl-val-cons->lst (erl-state->in s)))) x)
+      (equal (erl-val-integer->val
+              (car (erl-val-cons->lst (erl-state->in s)))) x)
       
       ; Let's assume the result is well-formed
       (wf-state-p (apply-k s (cons k nil))))
@@ -393,5 +396,5 @@
       (erl-state->in (apply-k s (cons k nil)))
       (make-erl-val-integer 
         :val  (/ (* x (+ x 1)) 2))))
-  :disable (apply-k-of-sum-of-x apply-k-of-sum)
-  :use (:instance apply-k-of-sum-of-x))
+  :disable (apply-k-of-sum-of-nats-of-x apply-k-of-sum-of-nats)
+  :use (:instance apply-k-of-sum-of-nats-of-x))
