acl2/books/erl-arithmetic/top.lisp
@@ -1,4 +1,4 @@
 (in-package "ACL2")
 
 (include-book "add")
-(include-book "sum")
+(include-book "sum_of_nats")
