acl2/books/reduce-v2/examples.lisp
@@ -1,0 +1,41 @@
+(in-package "ACL2")
+(include-book "wtree/create-wtree/top")
+
+
+; helper to print the leaf values.
+(local (define print-omap-values ((n network-p))
+  :measure (acl2-count (network-fix n))
+  (b* ((n (network-fix n))
+       ((if (omap::emptyp n)) 'ok)
+       (val (erl-state->in (proc->s (omap::head-val n))))
+       (- (cw "~x0~%" val)))
+    (print-omap-values (omap::tail n)))))
+
+
+; Reduce network with 10 processes.
+; Run the processes for 40 steps and print the results.
+; Remark: index starts at 0, so this one is a sum until n-1
+#| 
+  (print-omap-values (erl-runner (create-wtree 10) 40))
+|#
+
+
+; Reduce network with 100 processes.
+; Run the processes for 400 steps and print the results.
+; Remark: index starts at 0, so this one is a sum until n-1
+#| 
+  (print-omap-values (erl-runner (create-wtree 100) 400))
+|#
+
+; Reduce network with 1000 processes.
+; Run the processes for 4000 steps and print the results.
+; Remarks:
+; - index starts at 0, so this one is a sum until n-1
+; - there are a lot of processes, so it is better to
+;   just print the head.
+#|
+  (erl-state->in
+    (proc->s
+        (omap::head-val
+            (erl-runner (create-wtree 1000) 4000))))
+|#
